Isabelle2/BallotArrays3.thy
@@ -7,6 +7,35 @@ begin
 text {* A ballot array represents a history of execution of a Paxos-like algorithm, i.e. the current 
   ballot of every acceptor, and the history of all votes ever cast by every acceptor . *}
 
+text {* What about defining a new command to make type copies? *}
+
+typedef bal = "UNIV::nat set"
+by auto
+setup_lifting type_definition_bal
+lift_definition bal_zero :: bal is "0::nat" . 
+lift_definition bal_less_eq :: "bal \<Rightarrow> bal \<Rightarrow> bool" is less_eq .
+lift_definition bal_less :: "bal \<Rightarrow> bal \<Rightarrow> bool" is less .
+lift_definition bal_Suc :: "bal \<Rightarrow> bal" is Suc .
+instantiation bal :: zero
+begin
+definition zero_bal:
+  "0 = bal_zero"
+instance ..
+end
+instantiation bal :: ord
+begin
+definition less_eq_bal:"less_eq = bal_less_eq"
+definition less_bal:"less = bal_less"
+instance proof qed
+end
+instantiation bal :: linorder
+begin
+instance
+apply (intro_classes)
+apply ((simp only:less_bal less_eq_bal, transfer, force)+)
+done
+end
+
 locale ballot_array =
   fixes quorums :: "'a set set"
   and ballot :: "'a \<Rightarrow> nat"
@@ -26,9 +55,9 @@ definition conservative_array where
 
 text {* Here the @{term Max} is the one from @{text Lattices_Big} *}
 
-definition proved_safe_at_2_a where
+definition proved_safe_at_abs where
   -- {* Any value that has been proved safe at ballot b can be voted for in ballot b. *}
-  "proved_safe_at_2_a q b v \<equiv>
+  "proved_safe_at_abs q b v \<equiv>
     q \<in> quorums \<and> (\<forall> a \<in> q . ballot a \<ge> b) \<and>
     (if \<exists> a \<in> q . \<exists> b\<^sub>2 . b\<^sub>2 < b \<and> vote a b\<^sub>2 \<noteq> None
     then \<exists> a \<in> q . vote a (Max {b\<^sub>2 . \<exists> a \<in> q . b\<^sub>2 < b \<and> vote a b\<^sub>2 \<noteq> None}) = Some v
@@ -58,5 +87,19 @@ definition well_formed where
   "well_formed \<equiv> \<forall> a b . ballot a < b \<longrightarrow> vote a b = None"
 
 end
+
+term ballot_array.conservative
+term ballot_array.proved_safe_at_abs
+term ballot_array.conservative_array
+term ballot_array.chosen
+lift_definition bal_conservative :: "('a \<Rightarrow> bal \<Rightarrow> 'b option) \<Rightarrow> bal \<Rightarrow> bool" 
+  is ballot_array.conservative .
+lift_definition bal_proved_safe_at_abs 
+  :: "'a set set \<Rightarrow> ('a \<Rightarrow> bal) \<Rightarrow> ('a \<Rightarrow> bal \<Rightarrow> 'b option) \<Rightarrow> 'a set \<Rightarrow> bal \<Rightarrow> 'b \<Rightarrow> bool"
+  is ballot_array.proved_safe_at_abs .
+lift_definition bal_conservative_array :: "('a \<Rightarrow> bal \<Rightarrow> 'b option) \<Rightarrow> bool"
+  is ballot_array.conservative_array .
+lift_definition bal_chosen :: "'a set set \<Rightarrow> ('a \<Rightarrow> bal \<Rightarrow> 'b option) \<Rightarrow> 'b \<Rightarrow> bool"
+  is ballot_array.chosen .
 
 end
